Sketch Letrec case (yuck!)

compiler/backend/passes/proofs/env_to_stateProofScript.sml
@@ -15,7 +15,7 @@ local open pure_semanticsTheory in end
 val _ = new_theory "env_to_stateProof";
 
 val _ = set_grammar_ancestry
-  ["env_to_state_1Proof", "env_cexp", "state_cexp"];
+  ["env_to_state_1Proof", "env_cexp", "state_cexp", "state_unthunkProof"];
 
 Overload to_state = “env_to_state_1Proof$compile_rel”
 Overload unthunk = “state_unthunkProof$compile_rel”
@@ -35,6 +35,82 @@ Definition dest_Message_def:
   dest_Message (Message s) = SOME s ∧
   dest_Message _ = NONE
 End
+
+Definition Lets_def:
+  Lets [] x = (x:state_cexp$cexp) ∧
+  Lets ((v,y)::ys) x = Let v y (Lets ys x)
+End
+
+Definition Letrec_imm_def:
+  (Letrec_imm vs ((Var v):env_cexp$cexp) ⇔ MEM v vs) ∧
+  (Letrec_imm vs (Lam _ _) ⇔ T) ∧
+  (Letrec_imm vs _ ⇔ F)
+End
+
+Definition dest_Delay_def:
+  dest_Delay (Delay x) = SOME (x:env_cexp$cexp) ∧
+  dest_Delay _ = NONE
+End
+
+Definition dest_Lam_def:
+  dest_Lam (Lam v x) = SOME (v,x:env_cexp$cexp) ∧
+  dest_Lam _ = NONE
+End
+
+Definition Letrec_split_def:
+  Letrec_split vs [] = ([],[]) ∧
+  Letrec_split vs ((v:mlstring,x)::fns) =
+    let (xs,ys) = Letrec_split vs fns in
+      case dest_Delay x of
+      | SOME y => ((v,Letrec_imm vs y,y)::xs,ys)
+      | NONE =>
+        case dest_Lam x of
+        | SOME (n,z) => (xs,(v,n,z)::ys)
+        | NONE => (xs,ys)
+End
+
+Definition Bool_def[simp]:
+  Bool T = (True  :state_cexp$cexp) ∧
+  Bool F = (False :state_cexp$cexp)
+End
+
+Definition some_ref_bool_def:
+  some_ref_bool (v:mlstring,b,y:state_cexp$cexp) =
+    (SOME v, App Ref [Bool b; Bool b])
+End
+
+Definition unsafe_update_def:
+  unsafe_update (v,b,y) =
+    (NONE:mlstring option, App UnsafeUpdate [Var v; IntLit 1; if b then y else Lam NONE y])
+End
+
+Triviality Letrec_split_MEM_funs:
+  ∀xs delays funs m n x.
+    (delays,funs) = Letrec_split ns xs ∧ MEM (m,n,x) funs ⇒
+    cexp_size x ≤ list_size (pair_size mlstring_size cexp_size) xs
+Proof
+  Induct \\ fs [Letrec_split_def]
+  \\ PairCases \\ fs [Letrec_split_def] \\ rw []
+  \\ pairarg_tac \\ fs []
+  \\ gvs [AllCaseEqs()]
+  \\ res_tac \\ fs []
+  \\ fs [list_size_def,basicSizeTheory.pair_size_def]
+  \\ Cases_on ‘h1’ \\ gvs [dest_Lam_def,env_cexpTheory.cexp_size_def]
+QED
+
+Triviality Letrec_split_MEM_delays:
+  ∀xs delays funs m n x.
+    (delays,funs) = Letrec_split ns xs ∧ MEM (m,n,x) delays ⇒
+    cexp_size x ≤ list_size (pair_size mlstring_size cexp_size) xs
+Proof
+  Induct \\ fs [Letrec_split_def]
+  \\ PairCases \\ fs [Letrec_split_def] \\ rw []
+  \\ pairarg_tac \\ fs []
+  \\ gvs [AllCaseEqs()]
+  \\ res_tac \\ fs []
+  \\ fs [list_size_def,basicSizeTheory.pair_size_def]
+  \\ Cases_on ‘h1’ \\ gvs [dest_Delay_def,env_cexpTheory.cexp_size_def]
+QED
 
 Definition to_state_def:
   to_state ((Var n):env_cexp$cexp) = (Var n):state_cexp$cexp ∧
@@ -59,6 +135,13 @@ Definition to_state_def:
          Let NONE (App UnsafeUpdate [Var «v»; IntLit 0; True]) $
          Let NONE (App UnsafeUpdate [Var «v»; IntLit 1; Var «wh»]) $
            Var «wh») ∧
+  to_state (Letrec xs y) =
+    (let (delays,funs) = Letrec_split (MAP FST xs) xs in
+     let delays = MAP (λ(m,n,x). (m,n,to_state x)) delays in
+     let funs = MAP (λ(m,n,x). (m,n,to_state x)) funs in
+       Lets (MAP some_ref_bool delays) $
+       Letrec funs $
+       Lets (MAP unsafe_update delays) (to_state y)) ∧
   to_state (Let vo x y) =
     Let vo (to_state x) (to_state y) ∧
   to_state (If x y z) =
@@ -75,6 +158,9 @@ Definition to_state_def:
        | _ => App (AtomOp b) ys)
 Termination
   WF_REL_TAC ‘measure cexp_size’
+  \\ fs [env_cexpTheory.cexp_size_eq] \\ rw []
+  \\ (drule_all Letrec_split_MEM_delays ORELSE drule_all Letrec_split_MEM_funs)
+  \\ fs []
 End
 
 Definition compile_def:
@@ -93,6 +179,7 @@ Definition cexp_wf_def[simp]:
   cexp_wf (App x y) = (cexp_wf x ∧ cexp_wf y) ∧
   cexp_wf (Letrec fs x) =
     (EVERY I (MAP (λ(_,x). cexp_wf x) fs) ∧ cexp_wf x ∧
+     ALL_DISTINCT (MAP (λx. explode (FST x)) fs) ∧
      EVERY (λ(_,x). ∃n m. x = Lam n m ∨ x = Delay m) fs) ∧
   cexp_wf (Case x v rs) =
     (EVERY I (MAP (λ(_,_,x). cexp_wf x) rs) ∧ cexp_wf x ∧
@@ -203,9 +290,77 @@ Proof
   \\ irule to_state_lets_for \\ fs []
 QED
 
+Inductive thunk_res:
+  (∀x s. thunk_res ((Lam s x):stateLang$exp)) ∧
+  (∀x. thunk_res (App Ref [False; Lam NONE x]))
+End
+
+Definition inv_thunk_def:
+  inv_thunk (App Ref [False; Lam NONE x]) = Delay x ∧
+  inv_thunk (Lam s x) = Lam s x
+End
+
+Theorem imp_letrec_rel:
+  ∀xs xs0 ys.
+    (∀p_1 p_2. MEM (p_1,p_2) xs ⇒ ∃n m. p_2 = Lam n m ∨ p_2 = Delay m) ∧
+    LIST_REL unthunk xs0 ys ∧
+    LIST_REL to_state (MAP (λx. exp_of (SND x)) xs) xs0 ⇒
+    LIST_REL state_unthunkProof$letrec_rel xs0 (MAP inv_thunk ys) ∧
+    EVERY thunk_res ys
+Proof
+  Induct >- fs []
+  \\ Cases_on ‘xs0’ \\ fs [PULL_EXISTS]
+  \\ PairCases \\ simp []
+  \\ rpt gen_tac
+  \\ rpt $ disch_then assume_tac \\ fs []
+  \\ last_x_assum $ drule_at $ Pos last
+  \\ disch_then $ drule_at $ Pos last
+  \\ impl_tac >- metis_tac []
+  \\ strip_tac \\ simp []
+  \\ last_x_assum $ qspecl_then [‘h'0’,‘h'1’] mp_tac
+  \\ simp []
+  \\ strip_tac \\ gvs []
+  \\ qpat_x_assum ‘to_state _ _’ mp_tac
+  \\ simp [Once env_to_state_1ProofTheory.compile_rel_cases]
+  \\ strip_tac \\ gvs []
+  \\ last_x_assum mp_tac
+  \\ simp [Once state_unthunkProofTheory.compile_rel_cases]
+  \\ strip_tac \\ gvs []
+  \\ simp [Once thunk_res_cases,inv_thunk_def]
+  \\ simp [Once state_unthunkProofTheory.compile_rel_cases]
+QED
+
+Theorem clean_Lets:
+  ∀xs ys x y.
+    clean x y ∧ MAP FST xs = MAP FST ys ∧
+    LIST_REL clean (MAP SND xs) (MAP SND ys) ⇒
+    clean (Lets xs x) (Lets ys y)
+Proof
+  Induct \\ Cases_on ‘ys’ \\ fs [Lets_def]
+  \\ PairCases_on ‘h’ \\ PairCases \\ fs [Lets_def] \\ rw []
+  \\ irule_at Any state_app_unitProofTheory.cexp_rel_Let \\ fs []
+QED
+
+Theorem case_rel_Lets:
+  ∀xs ys x y.
+    MAP (OPTION_MAP explode o FST) xs = MAP FST ys ∧
+    LIST_REL case_rel (MAP exp_of (MAP SND xs)) (MAP SND ys) ∧
+    case_rel (exp_of x) y ⇒
+    case_rel (exp_of (Lets xs x)) (Lets ys y)
+Proof
+  Induct \\ Cases_on ‘ys’ \\ fs []
+  \\ fs [state_unthunkProofTheory.Lets_def,Lets_def]
+  \\ PairCases \\ PairCases_on ‘h’
+  \\ fs [state_unthunkProofTheory.Lets_def,Lets_def]
+  \\ rw []
+  \\ irule_at Any state_caseProofTheory.compile_rel_Let
+  \\ fs []
+QED
+
 Theorem to_state_rel:
   ∀x. cexp_wf x ⇒ combined x (to_state x)
 Proof
+
   ho_match_mp_tac to_state_ind \\ rpt strip_tac
   >~ [‘Var’] >-
    (rw [to_state_def,combined_def]
@@ -392,13 +547,160 @@ Proof
 
    (rw [to_state_def] \\ fs [combined_def]
     \\ rpt $ irule_at Any env_to_state_1ProofTheory.compile_rel_Letrec
+    \\ pairarg_tac \\ gvs []
+    \\ gvs [EVERY_MEM,SF ETA_ss,FORALL_PROD,MEM_MAP,PULL_EXISTS]
     \\ fs [MAP_MAP_o,combinTheory.o_DEF,UNCURRY]
-
-
-
-
-
-    \\ cheat)
+    \\ last_x_assum $ irule_at Any
+    \\ rpt $ irule_at Any state_unthunkProofTheory.compile_rel_Letrec
+    \\ last_x_assum $ irule_at Any
+    \\ ‘∀x. MEM x (MAP SND xs) ⇒
+            ∃x1 x2 y1.
+              to_state (exp_of x) x1 ∧ unthunk x1 x2 ∧
+              case_rel (exp_of y1) x2 ∧ clean y1 (to_state x)’ by
+      (rename [‘Letrec_split ts’]
+       \\ rpt $ pop_assum mp_tac
+       \\ qid_spec_tac ‘delays’
+       \\ qid_spec_tac ‘funs’
+       \\ qid_spec_tac ‘xs’
+       \\ Induct >- fs []
+       \\ PairCases
+       \\ simp_tac (srw_ss()) [Letrec_split_def,SF DNF_ss]
+       \\ rpt conj_tac
+       \\ qid_spec_tac ‘h1’ \\ simp_tac (srw_ss()) [dest_Delay_def,dest_Lam_def]
+       \\ Cases_on ‘Letrec_split ts xs’ \\ simp_tac (srw_ss()) [LET_THM]
+       \\ simp_tac (srw_ss()) [Letrec_split_def,SF DNF_ss]
+       \\ rpt strip_tac
+       THENL [all_tac, last_x_assum irule \\ metis_tac [],
+              all_tac, last_x_assum irule \\ metis_tac []]
+       \\ last_x_assum kall_tac \\ gvs []
+       \\ fs [to_state_def]
+       >-
+        (simp [Once env_to_state_1ProofTheory.compile_rel_cases,PULL_EXISTS]
+         \\ simp [Once state_unthunkProofTheory.compile_rel_cases,PULL_EXISTS]
+         \\ first_x_assum $ irule_at $ Pos hd
+         \\ first_x_assum $ irule_at $ Pos hd
+         \\ rpt $ irule_at Any state_app_unitProofTheory.cexp_rel_Lam \\ fs [PULL_EXISTS]
+         \\ first_x_assum $ irule_at $ Pos hd
+         \\ simp [Once state_caseProofTheory.compile_rel_cases,PULL_EXISTS])
+       \\ rpt $ irule_at Any state_app_unitProofTheory.cexp_rel_App \\ fs [PULL_EXISTS]
+       \\ rpt $ irule_at Any state_app_unitProofTheory.cexp_rel_App \\ fs [PULL_EXISTS]
+       \\ rpt $ irule_at Any state_app_unitProofTheory.cexp_rel_Lam \\ fs [PULL_EXISTS]
+       \\ rpt $ irule_at Any env_to_state_1ProofTheory.compile_rel_Delay
+       \\ first_x_assum $ irule_at $ Pos hd
+       \\ first_x_assum $ irule_at $ Pos hd
+       \\ rpt $ irule_at Any state_unthunkProofTheory.compile_rel_Delay \\ fs [PULL_EXISTS]
+       \\ first_x_assum $ irule_at $ Pos hd
+       \\ rpt $ irule_at Any state_caseProofTheory.compile_rel_App \\ fs [PULL_EXISTS]
+       \\ rpt $ irule_at Any state_caseProofTheory.compile_rel_App \\ fs [PULL_EXISTS]
+       \\ simp [Once state_caseProofTheory.compile_rel_cases])
+    \\ dxrule MEM_combined
+    \\ strip_tac
+    \\ simp_tac std_ss [Once SWAP_EXISTS_THM]
+    \\ qexists_tac ‘ZIP (MAP (λx. explode (FST x)) xs,xs0)’
+    \\ imp_res_tac LIST_REL_LENGTH \\ gvs []
+    \\ gvs [MAP_ZIP] \\ fs [MAP_MAP_o,combinTheory.o_DEF]
+    \\ drule_all imp_letrec_rel
+    \\ strip_tac
+    \\ imp_res_tac LIST_REL_LENGTH \\ gvs []
+    \\ simp_tac std_ss [Once SWAP_EXISTS_THM]
+    \\ qexists_tac ‘ZIP (MAP (λx. explode (FST x)) xs,MAP inv_thunk ys)’
+    \\ simp [comp_Letrec_def]
+    \\ gvs [MAP_ZIP]
+    \\ pairarg_tac \\ fs []
+    \\ ‘∃ds fs.
+          LIST_REL case_rel (MAP exp_of ds) (MAP (SND o SND) delays') ∧
+          LIST_REL case_rel (MAP exp_of fs) (MAP SND funs') ∧
+          LIST_REL clean ds (MAP (to_state o SND o SND) delays) ∧
+          LIST_REL clean fs (MAP (to_state o SND o SND) funs)’ by cheat
+    \\ qabbrev_tac ‘ds1 = MAP (λ((m,n,_),x). (m,n,x)) (ZIP (delays,ds))’
+    \\ qabbrev_tac ‘fs1 = MAP (λ((m,n,_),x). (m,n,x)) (ZIP (funs,fs))’
+    \\ qexists_tac ‘Lets (MAP some_ref_bool ds1) $
+                    Letrec fs1 $ Lets (MAP unsafe_update ds1) y1’
+    \\ reverse conj_tac
+    >-
+     (irule_at Any clean_Lets
+      \\ irule_at Any state_app_unitProofTheory.cexp_rel_Letrec \\ fs []
+      \\ irule_at Any clean_Lets
+      \\ fs []
+      \\ fs [Abbr‘fs1’,Abbr‘ds1’]
+      \\ ntac 2 $ pop_assum mp_tac
+      \\ qid_spec_tac ‘fs’
+      \\ qid_spec_tac ‘funs’
+      \\ qid_spec_tac ‘ds’
+      \\ qid_spec_tac ‘delays’
+      \\ rpt $ pop_assum kall_tac
+      \\ reverse Induct \\ Cases_on ‘ds’ \\ fs []
+      >-
+       (fs [] \\ rpt gen_tac \\ rpt $ disch_then strip_assume_tac
+        \\ last_x_assum drule_all \\ fs []
+        \\ PairCases_on ‘h'’ \\ fs [some_ref_bool_def,unsafe_update_def]
+        \\ fs [] \\ rpt gen_tac \\ rpt $ disch_then strip_assume_tac
+        \\ rpt (irule_at Any state_app_unitProofTheory.cexp_rel_App \\ fs [PULL_EXISTS])
+        \\ rpt (irule_at Any state_app_unitProofTheory.cexp_rel_Var \\ fs [PULL_EXISTS])
+        \\ Cases_on ‘h'1’ \\ fs []
+        \\ rpt (irule_at Any state_app_unitProofTheory.cexp_rel_App \\ fs [PULL_EXISTS])
+        \\ rpt (irule_at Any state_app_unitProofTheory.cexp_rel_Lam \\ fs [PULL_EXISTS]))
+      \\ reverse Induct \\ Cases_on ‘fs’ \\ fs []
+      \\ PairCases \\ fs [some_ref_bool_def,unsafe_update_def])
+    \\ irule_at Any case_rel_Lets \\ fs []
+    \\ ‘MAP (explode o FST) delays = MAP FST delays'’ by cheat
+    \\ ‘MAP (FST o SND) delays = MAP (FST o SND) delays'’ by cheat
+    \\ ‘MAP (explode o FST) funs = MAP FST funs'’ by cheat
+    \\ unabbrev_all_tac
+    \\ conj_tac
+    >-
+     (ntac 5 $ pop_assum mp_tac
+      \\ rpt $ pop_assum kall_tac
+      \\ qid_spec_tac ‘ds’
+      \\ qid_spec_tac ‘delays’
+      \\ qid_spec_tac ‘delays'’
+      \\ Induct \\ Cases_on ‘ds’ \\ Cases_on ‘delays’ \\ fs []
+      \\ PairCases_on ‘h'’ \\ PairCases \\ fs []
+      \\ fs [some_ref_bool_def,state_unthunkProofTheory.some_ref_bool_def])
+    \\ reverse conj_tac
+    >-
+     (ntac 5 $ pop_assum mp_tac
+      \\ rpt $ pop_assum kall_tac
+      \\ qid_spec_tac ‘ds’
+      \\ qid_spec_tac ‘delays’
+      \\ qid_spec_tac ‘delays'’
+      \\ Induct \\ Cases_on ‘ds’ \\ Cases_on ‘delays’ \\ fs []
+      \\ PairCases_on ‘h'’ \\ PairCases \\ fs []
+      \\ fs [some_ref_bool_def,state_unthunkProofTheory.some_ref_bool_def]
+      \\ rw [] \\ rename [‘Bool bb’] \\ Cases_on ‘bb’ \\ fs []
+      \\ rpt $ irule_at Any state_caseProofTheory.compile_rel_App \\ fs [PULL_EXISTS]
+      \\ rpt $ irule_at Any state_caseProofTheory.compile_rel_App \\ fs [PULL_EXISTS])
+    \\ rpt $ irule_at Any state_caseProofTheory.compile_rel_Letrec
+    \\ ntac 2 (conj_tac >-
+     (ntac 5 $ pop_assum mp_tac
+      \\ rpt $ pop_assum kall_tac
+      \\ qid_spec_tac ‘fs’
+      \\ qid_spec_tac ‘funs’
+      \\ qid_spec_tac ‘funs'’
+      \\ Induct \\ Cases_on ‘fs’ \\ Cases_on ‘funs’ \\ fs []
+      \\ PairCases_on ‘h'’ \\ PairCases \\ fs []))
+    \\ reverse conj_tac >-
+     (ntac 6 $ pop_assum mp_tac
+      \\ rpt $ pop_assum kall_tac
+      \\ qid_spec_tac ‘fs’
+      \\ qid_spec_tac ‘funs’
+      \\ qid_spec_tac ‘funs'’
+      \\ Induct \\ Cases_on ‘fs’ \\ Cases_on ‘funs’ \\ fs []
+      \\ PairCases_on ‘h'’ \\ PairCases \\ fs [] \\ cheat (* problem *))
+    \\ irule_at Any case_rel_Lets \\ fs []
+    \\ ntac 7 $ pop_assum mp_tac
+    \\ rpt $ pop_assum kall_tac
+    \\ qid_spec_tac ‘ds’
+    \\ qid_spec_tac ‘delays’
+    \\ qid_spec_tac ‘delays'’
+    \\ Induct \\ Cases_on ‘ds’ \\ Cases_on ‘delays’ \\ fs []
+    \\ PairCases_on ‘h'’ \\ PairCases \\ fs []
+    \\ fs [unsafe_update_def,state_unthunkProofTheory.unsafe_update_def]
+    \\ rw []
+    \\ rpt $ irule_at Any state_caseProofTheory.compile_rel_App \\ fs [PULL_EXISTS]
+    \\ rpt $ irule_at Any state_caseProofTheory.compile_rel_App \\ fs [PULL_EXISTS]
+    \\ rpt $ irule_at Any state_caseProofTheory.compile_rel_Var
+    \\ simp [Once state_caseProofTheory.compile_rel_cases])
 
   >~ [‘Prim (Cons m) xs’] >-
    (rw [to_state_def] \\ fs [combined_def]
@@ -437,7 +739,6 @@ Proof
     \\ rpt (irule_at Any state_unthunkProofTheory.compile_rel_Var \\ fs [PULL_EXISTS])
     \\ rpt (irule_at Any state_caseProofTheory.compile_rel_App \\ fs [PULL_EXISTS])
     \\ rpt (irule_at Any state_caseProofTheory.compile_rel_Var \\ fs [PULL_EXISTS]))
-  \\ cheat
 QED
 
 Theorem itree_of_to_state:
